lakefile.lean
@@ -138,3 +138,6 @@ lean_lib ZipTest where
 @[default_target]
 lean_exe test where
   root := `ZipTest
+
+lean_exe perfspike where
+  root := `PerfSpike
